LeanPy/Data/Dict/Object.lean
@@ -1,0 +1,165 @@
+/-
+Copyright (c) 2025 Mac Malone. All rights reserved.
+Released under the Apache 2.0 license as described in the file LICENSE.
+Authors: Mac Malone
+-/
+import LeanPy.Data.Object.Slots
+import LeanPy.Data.Str.Object
+
+namespace LeanPy
+
+/- An instance of a subclass of `dict` that satisfies `p`. -/
+abbrev PDictObject (p : ObjectProp) := PSubObject p dictTypeRef
+
+/- An instance of a subclass of `dict`. -/
+def DictObject := PDictObject .Any
+
+/-- Returns whether this object is an instance of a subtype of `dict`. -/
+@[inline] def Object.isDict (self : Object) : Bool :=
+ self.ty.isDictSubclass
+
+/-- Casts `self` to `DictObject`. -/
+@[inline] def Object.asDict (self : Object) (h : self.isDict) : DictObject :=
+  self.asSubObject (self.ty.isDictSubclass_iff_subset.mp h)
+
+/--
+Casts `self` to `DictObject` if `self` is instance of a subtype of `dict`.
+Otherwise, returns `none`.
+-/
+@[inline] def Object.asDict? (self : Object) : Option DictObject :=
+  if h : self.isDict then some (self.asDict h) else none
+
+namespace ObjectData -- replace with something more sound
+
+@[inline] private unsafe def ofDictImpl (dict : Dict) : ObjectData :=
+  unsafeCast dict
+
+@[implemented_by ofDictImpl]
+abbrev ofDict (dict : Dict) : ObjectData := .mkCore dictDataKind dict
+
+opaque getDict (self : ObjectData) (h : self.kind = dictDataKind) : Dict :=
+  unsafe unsafeCast self
+
+end ObjectData
+
+namespace Dict
+
+/--
+Returns `true` if the two dictionaries are equal.
+
+Dictionaries compare equal if and only if they have the same
+`(key, value)` pairs (regardless of ordering).
+-/
+-- Should follow the logic in CPython's `dict_equal`
+-- https://github.com/python/cpython/blob/3.11/Objects/dictobject.c#L3155
+def beqM (a b : Dict) : PyM Bool := do
+  let a ← a.get
+  let b ← b.get
+  unless a.size == b.size do
+    return false
+  for entry in a.entries do
+    let .some ah ak av := entry
+      | continue
+    let ⟨bi⟩ ← b.raw.getEntryIdxCoreM ah (.up <$> ak.beqM ·)
+    let some (.some _ _ bv) := b.entries[bi]?
+      | return false
+    let av ← av.get
+    let bv ← bv.get
+    unless (← av.beqM bv) do
+      return false
+  return true
+
+/-- Returns a string representation of the dictionary. -/
+-- Should follow the logic in CPython's `dict_repr`
+-- https://github.com/python/cpython/blob/3.11/Objects/dictobject.c#L2403
+def reprM (self : Dict) : PyM String := do
+  return (← appendHead "{" 0 (← self.get).entries).push '}'
+where
+  appendHead s i entries : PyM String := do
+    if h : i < entries.size then
+      if let .some _ k v := entries[i] then
+        appendTail (← append s k v) (i+1) entries
+      else appendHead s (i+1) entries
+    else return s
+  termination_by entries.size - i
+  decreasing_by omega
+  appendTail s i entries := do
+    if h : i < entries.size then
+      if let .some _ k v := entries[i] then
+        appendTail (← append s!"{s}, " k v) (i+1) entries
+      else appendTail s (i+1) entries
+    else return s
+  termination_by entries.size - i
+  decreasing_by all_goals omega
+  append s k v := do
+    let k ← k.reprM
+    let v ← (← v.get).reprM
+    return s!"{s}{k}: {v}"
+
+end Dict
+
+namespace DictObject
+
+instance : Coe DictObject Object := ⟨PObject.toObject⟩
+
+theorem isDict_toObject (self : DictObject) : self.toObject.isDict :=
+  self.ty.isDictSubclass_iff_subset.mpr self.ty_subset
+
+@[inline] def getDict (self : DictObject) : Dict :=
+  self.data.getDict (self.lawful_subobject).2
+
+/--
+Returns `true` if the two dictionaries are equal.
+
+This is equivalent to the Python `dict.__eq__(self, other)`.
+-/
+@[inline] protected def beqM (self other : DictObject) : PyM Bool :=
+  self.getDict.beqM other.getDict
+
+/--
+Returns `true` if the two dictionaries are not equal.
+
+This is equivalent to the Python `dict.__ne__(self, other)`.
+-/
+@[inline] protected def bneM (self other : DictObject) : PyM Bool :=
+  not <$> self.beqM other
+
+/--
+Return the number of items in the dictionary.
+
+This is equivalent to the Python `dict.len(self)`.
+-/
+@[inline] def lengthM (self : DictObject) : BaseIO Nat :=
+  (·.size) <$> self.getDict.get
+
+/-- Return `true` unless the dictionary is empty. -/
+@[inline] def toBoolM (self : DictObject) : BaseIO Bool :=
+  (· != 0) <$> self.lengthM
+
+/--
+Return a string representation of the dictionary.
+
+This is equivalent to the Python `dict.__repr__(self)`.
+-/
+@[inline] def reprM (self : DictObject) : PyM String :=
+  self.getDict.reprM
+
+end DictObject
+
+def dictTypeRef.slots : TObjectSlots DictObject where
+  hash _ := do -- TODO: make a TypeError & build this into the slot
+    throw ((← mkStrObject "unhashable type: 'dict'") : ErrorObject)
+  beq self other :=
+    if let some other := other.asDict? then self.beqM other else return false
+  bne self other :=
+    if let some other := other.asDict? then self.beqM other else return true
+  bool self := self.toBoolM
+  repr self := self.reprM
+
+@[instance] initialize dictTypeSlotsRef : TypeSlots dictTypeRef ←
+  dictTypeRef.slots.mkRef
+
+@[inline] def DictObject.ofDict (r : Dict) : DictObject :=
+  dictTypeRef.mkObjectCore r.id  (.ofDict r)
+
+instance : Coe Dict DictObject := ⟨DictObject.ofDict⟩
