LeanPy/Data/Dict/TypeRef.lean
@@ -1,0 +1,34 @@
+/-
+Copyright (c) 2025 Mac Malone. All rights reserved.
+Released under the Apache 2.0 license as described in the file LICENSE.
+Authors: Mac Malone
+-/
+import LeanPy.Data.Object.TypeRef
+
+namespace LeanPy
+
+def dictType.doc : String := "\
+  dict() -> new empty dictionary\n\
+  dict(mapping) -> new dictionary initialized from a mapping object's\n\
+      (key, value) pairs\n\
+  dict(iterable) -> new dictionary initialized as if via:\n\
+      d = {}\n\
+      for k, v in iterable:\n\
+          d[k] = v\n\
+  dict(**kwargs) -> new dictionary initialized with the name=value pairs\n\
+      in the keyword argument list.  For example:  dict(one=1, two=2)\
+  "
+
+-- TODO: replace with something more sound
+def dictDataKind : DataKind := `LeanPy.Dict
+
+@[reducible] def dictType : PyType where
+  name := "dict"
+  doc? := some dictType.doc
+  base? := some objectTypeRef
+  isDictSubclass := true
+  IsValidObject id data := id.isNonScalar ∧ data.kind = dictDataKind
+
+initialize dictTypeRef.init : InitTypeRef dictType ← initTypeRef
+
+abbrev dictTypeRef : TypeRef := dictTypeRef.init.toTypeRef
